Rename Generic files into HPKE.Interface

code/hpke/Hacl.HPKE.Interface.AEAD.fst
@@ -1,13 +1,19 @@
-module Hacl.Impl.Instantiate.AEAD
+module Hacl.HPKE.Interface.AEAD
 
 open FStar.HyperStack
 open FStar.HyperStack.All
 
 open Lib.Buffer
 
-module SAE = Spec.Agile.AEAD
-
 friend Spec.Agile.AEAD
+
+/// These two functions will never be extracted, they are only an interface
+/// boundary for the tactic performing instantiations.
+/// In other files, it is exposed as an assume val, but for AEAD, we need an fsti
+/// since we need to friend Spec.Agile.AEAD to perform the instantiations below,
+/// and assume val are forbidden in interface files
+let aead_encrypt #cs = admit()
+let aead_decrypt #cs = admit()
 
 #set-options "--z3rlimit 60 --fuel 0 --ifuel 0"
 
